.

theories/Prelude/PreludeUtil.v
@@ -239,7 +239,7 @@ Module NAT_FACTS.
     end
   .
 
-  Lemma le_iff {n : nat} {m : nat} :
+  Lemma le_unfold {n : nat} {m : nat} :
     n <= m <->
     match m with
     | O => n = 0
@@ -320,6 +320,15 @@ Module NAT_FACTS.
     }
   Qed.
 
+  Theorem lt_strong_ind {phi : nat -> Prop}
+    (ind_claim : forall n : nat, << IH : forall m : nat, m < n -> phi m >> -> phi n)
+    : forall n : nat, phi n.
+  Proof.
+    unnw. intros n. eapply ind_claim. induction n as [ | n IH].
+    - intros m. exact (@lt_elim_n_lt_0 (phi m) m).
+    - intros m hyp_m_lt_S_n. eapply ind_claim. intros i hyp_i_lt_m. eapply IH. exact (le_transitivity hyp_i_lt_m (lt_elim_n_lt_S_m hyp_m_lt_S_n)).
+  Defined.
+
   Inductive Le (n : nat) : nat -> Set :=
   | Le_n : Le n n
   | Le_S (m : nat) (hyp_Le : Le n m) : Le n (S m)
@@ -356,31 +365,6 @@ Module NAT_FACTS.
     | Le_S _ m' hyp_le' => le_S n m' (Le_implies_le hyp_le')
     end
   .
-
-  Lemma le_unfold {n : nat} {m : nat} (hyp_le : n <= m) :
-    match m with
-    | O => {_ : unit | n = 0}
-    | S m' => {n = S m'} + {n <= m'}
-    end.
-  Proof.
-    destruct m as [ | m'].
-    - exists (tt). exact (le_antisymmetry hyp_le le_intro_0_le_n).
-    - exact (
-        match le_implies_Le hyp_le in Le _ x return {n = x} + {n <= Nat.pred x} with
-        | Le_n _ => left (eq_reflexivity n)
-        | Le_S _ m' hyp_le' => right (Le_implies_le hyp_le')
-        end
-      ).
-  Defined.
-
-  Theorem lt_strong_ind {phi : nat -> Prop}
-    (ind_claim : forall n : nat, << IH : forall m : nat, m < n -> phi m >> -> phi n)
-    : forall n : nat, phi n.
-  Proof.
-    unnw. intros n. eapply ind_claim. induction n as [ | n IH].
-    - intros m. exact (@lt_elim_n_lt_0 (phi m) m).
-    - intros m hyp_m_lt_S_n. eapply ind_claim. intros i hyp_i_lt_m. eapply IH. exact (le_transitivity hyp_i_lt_m (lt_elim_n_lt_S_m hyp_m_lt_S_n)).
-  Defined.
 
 End NAT_FACTS.
 
@@ -656,6 +640,61 @@ Module FUN_FACTS.
     ; wfRel_well_founded := @lt_strong_ind (@Acc nat lt) (@Acc_intro nat lt)
     }
   .
+
+(*
+  Section LexicographicOrder. (* Reference: "https://github.com/agda/agda-stdlib/blob/456930d31e99ba1669a51a70e0d41e0434a9bb14/src/Induction/WellFounded.agda#L183" *)
+
+  Context {A : Type} {B : A -> Type}.
+
+  Let C : Type := @sigT A B.
+
+  Inductive sigT_wfRel (wfRel_A : A -> A -> Prop) (wfRel_B : forall x : A, B x -> B x -> Prop) : C -> C -> Prop :=
+  | sigT_wfRel_fst (x1 : A) (x2 : A) (y1 : B x1) (y2 : B x2)
+    (hyp_wfRel_x1_x2 : wfRel_A x1 x2)
+    : sigT_wfRel wfRel_A wfRel_B (@existT A B x1 y1) (@existT A B x2 y2)
+  | sigT_wfRel_snd (x : A) (y1 : B x) (y2 : B x)
+    (hyp_wfRel_y1_y2 : wfRel_B x y1 y2)
+    : sigT_wfRel wfRel_A wfRel_B (@existT A B x y1) (@existT A B x y2)
+  .
+
+  Lemma sigT_wfRel_well_founded_aux {wfRel_A : A -> A -> Prop} {wfRel_B : forall x : A, B x -> B x -> Prop}
+    (wf_A : forall x' : A, Acc wfRel_A x')
+    (wf_B : forall x' : A, forall y' : B x', Acc (wfRel_B x') y')
+    : forall root : C, Acc (sigT_wfRel wfRel_A wfRel_B) root.
+  Proof.
+    unnw. intros root.
+    pose proof (wf_A (projT1 root)) as acc_x.
+    pose proof (wf_B (projT1 root) (projT2 root)) as acc_y.
+    revert root acc_x acc_y.
+    refine (
+      fix to_show_fix (tree : C) (acc_tree1 : Acc wfRel_A (projT1 tree)) (acc_tree2 : Acc (wfRel_B (projT1 tree)) (projT2 tree)) : Acc (sigT_wfRel wfRel_A wfRel_B) tree :=
+      match acc_tree1, acc_tree2 with
+      | Acc_intro _ hyp_acc_root1, Acc_intro _ hyp_acc_root2 => _
+      end
+    ).
+    econstructor. intros subtree wfRel_subtree_tree. destruct wfRel_subtree_tree as [x1 x2 y1 y2 hyp_wfRel_x1_x2 | x y1 y2 hyp_wfRel_y1_y2].
+    - eapply to_show_fix with (tree := existT B x1 y1).
+      + eapply hyp_acc_root1. exact (hyp_wfRel_x1_x2).
+      + exact (wf_B x1 y1).
+    - eapply to_show_fix with (tree := existT B x y1).
+      + exact (wf_A x).
+      + eapply hyp_acc_root2. exact (hyp_wfRel_y1_y2).
+  Defined.
+
+  Hypothesis A_isWellFounded : isWellFounded A.
+
+  Hypothesis B_x_isWellFounded : forall x : A, isWellFounded (B x).
+
+  Definition indexed_lexicographical_order : C -> C -> Prop := sigT_wfRel (@wfRel A A_isWellFounded) (fun x : A => @wfRel (B x) (B_x_isWellFounded x)).
+
+  Global Instance pair_isWellFounded
+    : isWellFounded (@sigT A B).
+  Proof.
+    exists (indexed_lexicographical_order).
+  Defined.
+
+  End LexicographicOrder.
+*)
 
 End FUN_FACTS.
 
